ZxLean.lean
@@ -2,4 +2,5 @@
 -- Import modules here that should be built as part of the library.
 import ZxLean.ZXDiagram
 import ZxLean.ZXCalculus
+import ZxLean.Axioms
 import ZxLean.Visualize
